devel/Iron/Language/SystemF2Effect/SubstValExp.v
@@ -43,13 +43,16 @@ Proof.
    unfold liftTE. rewrite map_delete. eauto.
    eapply get_map. eauto.
    unfold liftTE. rewrite <- map_delete.
-    rrwrite (map (liftTT 1 0) (delete ix te) = liftTE 0 (delete ix te)). 
+    rrwrite ( map (liftTT 1 0) (delete ix te) 
+            = liftTE 0 (delete ix te)). 
     eauto using typev_kienv_weaken1.
 
  Case "XLet".
   apply TxLet; eauto.
    rewrite delete_rewind.
    eauto using typev_tyenv_weaken1.
+
+ 
 Qed.
 
 
