devel/Iron/Language/SystemF2Effect/VaExpBase.v
@@ -33,11 +33,16 @@ with     exp : Type :=
   | XApp    : val -> val -> exp
   | XAPP    : val -> ty  -> exp
 
+  (* Store operators *)
+  | XNew    : exp -> exp
+  | XUse    : nat -> exp -> exp
   | XAlloc  : ty  -> val -> exp
   | XRead   : ty  -> val -> exp
   | XWrite  : ty  -> val -> val -> exp
 
-  | XOp1    : op1 -> val -> exp.
+  (* Primitive operators *)
+  | XOp1   : op1 -> val -> exp.
+
 Hint Constructors val.
 Hint Constructors exp.
 
@@ -56,6 +61,8 @@ Lemma exp_mutind : forall
  -> (forall t x1 x2,    PX x1 -> PX x2          -> PX (XLet   t x1 x2))
  -> (forall v1 v2,      PV v1 -> PV v2          -> PX (XApp   v1 v2))
  -> (forall v t,        PV v                    -> PX (XAPP   v  t))
+ -> (forall x,          PX x                    -> PX (XNew   x))
+ -> (forall n x,        PX x                    -> PX (XUse   n x))
  -> (forall r v,        PV v                    -> PX (XAlloc r v))
  -> (forall r v,        PV v                    -> PX (XRead  r v))
  -> (forall r v1 v2,    PV v1 -> PV v2          -> PX (XWrite r v1 v2))
@@ -63,7 +70,9 @@ Lemma exp_mutind : forall
  ->  forall x, PX x.
 Proof. 
  intros PX PV.
- intros hVar hLoc hLam hLAM hConst hVal hLet hApp hAPP hAlloc hRead hWrite hOp1.
+ intros hVar hLoc hLam hLAM hConst hVal hLet hApp hAPP 
+        hNew hUse hAlloc hRead hWrite 
+        hOp1.
  refine (fix  IHX x : PX x := _
          with IHV v : PV v := _
          for  IHX).
@@ -74,6 +83,8 @@ Proof.
  apply hLet.   apply IHX. apply IHX.
  apply hApp.   apply IHV. apply IHV.
  apply hAPP.   apply IHV.
+ apply hNew.   apply IHX.
+ apply hUse.   apply IHX.
  apply hAlloc. apply IHV.
  apply hRead.  apply IHV.
  apply hWrite. apply IHV. apply IHV.
