devel/Iron/Language/SystemF2Effect/VaExpLift.v
@@ -20,6 +20,8 @@ Fixpoint liftTV (d: nat) (vv: val) : val :=
   |  XApp x1 x2   => XApp   (liftTV d x1)   (liftTV d x2)
   |  XAPP x t     => XAPP   (liftTV d x)    (liftTT 1 d t)
 
+  |  XNew x          => XNew   (liftTX (S d) x)
+  |  XUse n x        => XUse   n (liftTX d x)
   |  XAlloc tR v     => XAlloc (liftTT 1 d tR) (liftTV d v)
   |  XRead  tR v     => XRead  (liftTT 1 d tR) (liftTV d v)
   |  XWrite tR v1 v2 => XWrite (liftTT 1 d tR) (liftTV d v1) (liftTV d v2)
@@ -51,6 +53,8 @@ Fixpoint liftXV (n: nat) (d: nat) (vv: val) {struct vv} : val :=
   | XApp v1 v2   => XApp   (liftXV n d v1) (liftXV n d v2)
   | XAPP v1 t2   => XAPP   (liftXV n d v1) t2
 
+  | XNew x          => XNew   (liftXX n d x)
+  | XUse n2 x       => XUse   n2 (liftXX n d x)
   | XAlloc tR v     => XAlloc tR (liftXV n d v)
   | XRead  tR v     => XRead  tR (liftXV n d v)
   | XWrite tR v1 v2 => XWrite tR (liftXV n d v1) (liftXV n d v2)
